KA-CDP.ec
@@ -13,7 +13,6 @@ require BitWord FelTactic.
 require import BitVec.
 require CompDiffPriv KeyAgreement.
 
-op input_len : {int | 0 < input_len} as gt0_input_len.
 
 
 (* CDP for hamming distance *)
@@ -70,16 +69,16 @@ clone BitWord as CDPTransc with
     op n <- CDP_transc_len
 proof gt0_n by apply gt0_CDP_transc_len.
 
-type transcript = CDPTransc.word.
+type transc_CDP = CDPTransc.word.
 
 
 (* functionality of CDP *)
 
-op T_CDP : vec -> randA_CDP -> vec -> randB_CDP -> transcript.
+op T_CDP : vec -> randA_CDP -> vec -> randB_CDP -> transc_CDP.
 
-op outA_CDP : vec -> randA_CDP -> transcript -> int.
+op outA_CDP : vec -> randA_CDP -> transc_CDP -> int.
 
-op outB_CDP : vec -> randB_CDP -> transcript -> int.
+op outB_CDP : vec -> randB_CDP -> transc_CDP -> int.
 
 clone import CompDiffPriv as CDP with
     type input <- vec,
@@ -89,7 +88,7 @@ clone import CompDiffPriv as CDP with
     op drandA <- drandA_CDP,
     type randB <- randB_CDP,
     op drandB <- drandB_CDP,
-    type transcript <- transcript,
+    type transcript <- transc_CDP,
     op F <- hd,
     op adj <- adj,
     op T <- T_CDP,
@@ -106,3 +105,100 @@ realize drandB_fu. apply drandB_CDP_fu. qed.
 realize drandB_uni. apply drandB_CDP_uni. qed.
 realize drandB_ll. apply drandB_CDP_ll. qed.
 
+
+
+(* Key Agreement protocols *)
+
+type randA_KA = vec * vec * randA_CDP. 
+
+type randB_KA = vec * randB_CDP.
+
+type transc_KA = vec * vec * vec * transc_CDP.
+
+clone import KeyAgreement as KA with
+    type randA <- randA_KA,
+    type randB <- randB_KA,
+    type transcript <- transc_KA,
+    type key <- int.
+
+
+(* KA out of CDP for hd *)
+
+module KeyAgr : KA = {
+    var ra : randA_KA
+    var rb : randB_KA
+
+    proc init_A() : unit = {
+        var x, r : vec;
+        var ra_CDP : randA_CDP;
+        x <$ dvec;
+        r <$ dvec;
+        ra_CDP <$ drandA_CDP;
+        ra <- (x, r, ra_CDP);
+    }
+
+    proc init_B() : unit = {
+        var y : vec;
+        var rb_CDP : randB_CDP;
+        y <$ dvec;
+        rb_CDP <$ drandB_CDP;
+        rb <- (y, rb_CDP);
+    }
+    
+    proc exec() : transc_KA = {
+        var x, y, r, xr, yri : vec;
+        var ra_CDP : randA_CDP;
+        var rb_CDP : randB_CDP;
+        var tr_CDP : transc_CDP;
+        (x, r, ra_CDP) <- ra;
+        (y, rb_CDP) <- rb;
+        tr_CDP <- T_CDP x ra_CDP y rb_CDP;
+        xr <- andv x r;
+        yri <- andv y (invv r);
+        return (xr, r, yri, tr_CDP);
+    }
+
+    proc key_gen_A (tr : transc_KA) : int = {
+        var x, r, yri : vec;
+        var ra_CDP : randA_CDP;
+        var tr_CDP : transc_CDP;
+        var out : int;
+        (x, r, ra_CDP) <- ra;
+        yri <- tr.`3;
+        tr_CDP <- tr.`4;
+        out <- outA_CDP x ra_CDP tr_CDP;
+        return out - (hd (andv x (invv r)) yri);
+    }
+
+    proc key_gen_B (tr : transc_KA) : int = {
+        var y, r, xr: vec;
+        y <- rb.`1;
+        xr <- tr.`1;
+        r <- tr.`2;
+        return hd xr (andv y r);
+    }
+}.
+
+
+(* proving correctness of KA *)
+
+lemma correctness &m: Pr[Cor_CDP(CompDiffPriv).main() @ &m : res] <= Pr [Cor_KA(KeyAgr).main() @ &m : res].
+proof.
+byequiv => //; proc.
+inline{1}*.
+inline{2}*.
+auto.
+swap{1} 5 -2.
+swap{2} 4 1.
+auto.
+swap{2} 2 -1.
+swap{2} 3 1.
+rnd.
+rnd.
+rnd.
+auto.
+simplify.
+move => r _ xL _ yL _ raL _ rbL _ outA_CDP.
+rewrite outA_CDP.
+smt(subset_hd).
+qed.
